Finish porting rebind

Semantic/CC/Denotation/Rebind.lean
@@ -109,12 +109,12 @@ def rebind_shape_val_denot
       have hC := rebind_captureset_denot ρ T1.captureSet
       cases T1
       case capt C S =>
-        simp [Ty.captureSet] at hC hd ⊢
-        have ih2 := rebind_exi_exp_denot (ρ.liftVar (x:=arg)) T2
+        simp [Ty.captureSet, Ty.rename] at hC hd ⊢
+        have ih2 := rebind_exi_exp_denot (ρ.liftVar (x:=arg) (R:=reachability_of_loc H' arg)) T2
         have harg' := (ih1 _ _).mpr harg
         specialize hd arg H' hsub harg'
-        rw [hC] at hd ih2
-        exact (ih2 (A ∪ (C.rename f).denot env2 φ) H' _).mp hd
+        rw [hC] at hd
+        exact (ih2 (A ∪ (C.rename f).denot env2) H' _).mp hd
     · intro h
       obtain ⟨cs0, T0, t0, hr, hd⟩ := h
       use cs0, T0, t0
@@ -124,11 +124,11 @@ def rebind_shape_val_denot
       cases T1
       case capt C S =>
         simp [Ty.captureSet, Ty.rename] at hC hd ⊢
-        have ih2 := rebind_exi_exp_denot (ρ.liftVar (x:=arg)) T2
+        have ih2 := rebind_exi_exp_denot (ρ.liftVar (x:=arg) (R:=reachability_of_loc H' arg)) T2
         have harg' := (ih1 _ _).mp harg
         specialize hd arg H' hsub harg'
         rw [← hC] at hd
-        exact (ih2 (A ∪ C.denot env1 φ) H' _).mpr hd
+        exact (ih2 (A ∪ C.denot env1) H' _).mpr hd
   | .poly T1 T2 => by
     have ih1 := rebind_shape_val_denot ρ T1
     intro A s0 e0
@@ -140,7 +140,7 @@ def rebind_shape_val_denot
       apply And.intro hr
       intro H' denot hsub hproper himply
       have ih2 := rebind_exi_exp_denot (ρ.liftTVar (d:=denot)) T2
-      have himply' : denot.ImplyAfter H' (Ty.shape_val_denot env1 φ T1) := by
+      have himply' : denot.ImplyAfter H' (Ty.shape_val_denot env1 T1) := by
         intro H'' hsub' A' e hdenot
         exact (ih1 _ _ _).mpr (himply H'' hsub' A' e hdenot)
       specialize hd H' denot hsub hproper himply'
@@ -165,17 +165,19 @@ def rebind_shape_val_denot
       obtain ⟨cs0, B0, t0, hr, hd⟩ := h
       use cs0, B0, t0
       apply And.intro hr
-      intro H' A0 hsub hsub_bound
+      intro H' CS hsub hsub_bound
+      let A0 := CS.denot TypeEnv.empty
       have ih2 := rebind_exi_exp_denot (ρ.liftCVar (c:=A0)) T
-      specialize hd H' A0 hsub hsub_bound
+      specialize hd H' CS hsub hsub_bound
       exact (ih2 A H' _).mp hd
     · intro h
       obtain ⟨cs0, B0, t0, hr, hd⟩ := h
       use cs0, B0, t0
       apply And.intro hr
-      intro H' A0 hsub hsub_bound
+      intro H' CS hsub hsub_bound
+      let A0 := CS.denot TypeEnv.empty
       have ih2 := rebind_exi_exp_denot (ρ.liftCVar (c:=A0)) T
-      specialize hd H' A0 hsub hsub_bound
+      specialize hd H' CS hsub hsub_bound
       exact (ih2 A H' _).mpr hd
 
 def rebind_capt_val_denot
@@ -189,6 +191,7 @@ def rebind_capt_val_denot
     intro s e
     simp [Ty.capt_val_denot, Ty.rename]
     rw [← hC]
+    intro hwf
     exact hS (C.denot env1) s e
 
 def rebind_exi_val_denot
@@ -252,52 +255,52 @@ def rebind_exi_exp_denot
 
 end
 
--- def Rebind.weaken {env : TypeEnv s} {x : Nat} :
---   Rebind env Rename.succ (env.extend_var x) where
---   var := fun _ => rfl
+def Rebind.weaken {env : TypeEnv s} {x : Nat} {R : CapabilitySet} :
+  Rebind env Rename.succ (env.extend_var x R) where
+  var := fun _ => rfl
 
--- def Rebind.tweaken {env : TypeEnv s} {d : PreDenot} :
---   Rebind env Rename.succ (env.extend_tvar d) where
---   var := fun _ => rfl
+def Rebind.tweaken {env : TypeEnv s} {d : PreDenot} :
+  Rebind env Rename.succ (env.extend_tvar d) where
+  var := fun _ => rfl
 
--- def Rebind.cweaken {env : TypeEnv s} {c : CapabilitySet} :
---   Rebind env Rename.succ (env.extend_cvar c) where
---   var := fun _ => rfl
+def Rebind.cweaken {env : TypeEnv s} {c : CapabilitySet} :
+  Rebind env Rename.succ (env.extend_cvar c) where
+  var := fun _ => rfl
 
--- lemma weaken_shape_val_denot {env : TypeEnv s} {φ : HeapTopology} {T : Ty .shape s} :
---   Ty.shape_val_denot env φ T ≈ Ty.shape_val_denot (env.extend_var x) φ (T.rename Rename.succ) := by
---   apply rebind_shape_val_denot (ρ:=Rebind.weaken) (T:=T)
+lemma weaken_shape_val_denot {env : TypeEnv s} {T : Ty .shape s} :
+  Ty.shape_val_denot env T ≈ Ty.shape_val_denot (env.extend_var x R) (T.rename Rename.succ) := by
+  apply rebind_shape_val_denot (ρ:=Rebind.weaken) (T:=T)
 
--- lemma weaken_capt_val_denot {env : TypeEnv s} {φ : HeapTopology} {T : Ty .capt s} :
---   Ty.capt_val_denot env φ T ≈ Ty.capt_val_denot (env.extend_var x) φ (T.rename Rename.succ) := by
---   apply rebind_capt_val_denot (ρ:=Rebind.weaken) (T:=T)
+lemma weaken_capt_val_denot {env : TypeEnv s} {T : Ty .capt s} :
+  Ty.capt_val_denot env T ≈ Ty.capt_val_denot (env.extend_var x R) (T.rename Rename.succ) := by
+  apply rebind_capt_val_denot (ρ:=Rebind.weaken) (T:=T)
 
--- lemma weaken_exi_val_denot {env : TypeEnv s} {φ : HeapTopology} {T : Ty .exi s} :
---   Ty.exi_val_denot env φ T ≈ Ty.exi_val_denot (env.extend_var x) φ (T.rename Rename.succ) := by
---   apply rebind_exi_val_denot (ρ:=Rebind.weaken) (T:=T)
+lemma weaken_exi_val_denot {env : TypeEnv s} {T : Ty .exi s} :
+  Ty.exi_val_denot env T ≈ Ty.exi_val_denot (env.extend_var x R) (T.rename Rename.succ) := by
+  apply rebind_exi_val_denot (ρ:=Rebind.weaken) (T:=T)
 
--- lemma tweaken_shape_val_denot {env : TypeEnv s} {φ : HeapTopology} {T : Ty .shape s} :
---   Ty.shape_val_denot env φ T ≈ Ty.shape_val_denot (env.extend_tvar d) φ (T.rename Rename.succ) := by
---   apply rebind_shape_val_denot (ρ:=Rebind.tweaken) (T:=T)
+lemma tweaken_shape_val_denot {env : TypeEnv s} {T : Ty .shape s} :
+  Ty.shape_val_denot env T ≈ Ty.shape_val_denot (env.extend_tvar d) (T.rename Rename.succ) := by
+  apply rebind_shape_val_denot (ρ:=Rebind.tweaken) (T:=T)
 
--- lemma tweaken_capt_val_denot {env : TypeEnv s} {φ : HeapTopology} {T : Ty .capt s} :
---   Ty.capt_val_denot env φ T ≈ Ty.capt_val_denot (env.extend_tvar d) φ (T.rename Rename.succ) := by
---   apply rebind_capt_val_denot (ρ:=Rebind.tweaken) (T:=T)
+lemma tweaken_capt_val_denot {env : TypeEnv s} {T : Ty .capt s} :
+  Ty.capt_val_denot env T ≈ Ty.capt_val_denot (env.extend_tvar d) (T.rename Rename.succ) := by
+  apply rebind_capt_val_denot (ρ:=Rebind.tweaken) (T:=T)
 
--- lemma tweaken_exi_val_denot {env : TypeEnv s} {φ : HeapTopology} {T : Ty .exi s} :
---   Ty.exi_val_denot env φ T ≈ Ty.exi_val_denot (env.extend_tvar d) φ (T.rename Rename.succ) := by
---   apply rebind_exi_val_denot (ρ:=Rebind.tweaken) (T:=T)
+lemma tweaken_exi_val_denot {env : TypeEnv s} {T : Ty .exi s} :
+  Ty.exi_val_denot env T ≈ Ty.exi_val_denot (env.extend_tvar d) (T.rename Rename.succ) := by
+  apply rebind_exi_val_denot (ρ:=Rebind.tweaken) (T:=T)
 
--- lemma cweaken_shape_val_denot {env : TypeEnv s} {φ : HeapTopology} {T : Ty .shape s} :
---   Ty.shape_val_denot env φ T ≈ Ty.shape_val_denot (env.extend_cvar c) φ (T.rename Rename.succ) := by
---   apply rebind_shape_val_denot (ρ:=Rebind.cweaken) (T:=T)
+lemma cweaken_shape_val_denot {env : TypeEnv s} {T : Ty .shape s} :
+  Ty.shape_val_denot env T ≈ Ty.shape_val_denot (env.extend_cvar c) (T.rename Rename.succ) := by
+  apply rebind_shape_val_denot (ρ:=Rebind.cweaken) (T:=T)
 
--- lemma cweaken_capt_val_denot {env : TypeEnv s} {φ : HeapTopology} {T : Ty .capt s} :
---   Ty.capt_val_denot env φ T ≈ Ty.capt_val_denot (env.extend_cvar c) φ (T.rename Rename.succ) := by
---   apply rebind_capt_val_denot (ρ:=Rebind.cweaken) (T:=T)
+lemma cweaken_capt_val_denot {env : TypeEnv s} {T : Ty .capt s} :
+  Ty.capt_val_denot env T ≈ Ty.capt_val_denot (env.extend_cvar c) (T.rename Rename.succ) := by
+  apply rebind_capt_val_denot (ρ:=Rebind.cweaken) (T:=T)
 
--- lemma cweaken_exi_val_denot {env : TypeEnv s} {φ : HeapTopology} {T : Ty .exi s} :
---   Ty.exi_val_denot env φ T ≈ Ty.exi_val_denot (env.extend_cvar c) φ (T.rename Rename.succ) := by
---   apply rebind_exi_val_denot (ρ:=Rebind.cweaken) (T:=T)
+lemma cweaken_exi_val_denot {env : TypeEnv s} {T : Ty .exi s} :
+  Ty.exi_val_denot env T ≈ Ty.exi_val_denot (env.extend_cvar c) (T.rename Rename.succ) := by
+  apply rebind_exi_val_denot (ρ:=Rebind.cweaken) (T:=T)
 
--- end CC
+end CC
